theories/eio/rcfd__code.v
@@ -12,7 +12,7 @@ From zoo Require Import
 
 Definition rcfd_make : val :=
   fun: "fd" =>
-    { #0, ‘Open{ "fd" } }.
+    { #0, Reveal ‘Open( "fd" ) }.
 
 Definition rcfd_closed : val :=
   ‘Closing( fun: <> => () ).
