theories/language/proofmode.v
@@ -104,7 +104,7 @@ Section zoo_G.
     ( val_neq v1 v2 →
       envs_entails Δ' (WP fill K #false @ E {{ Φ }})
     ) →
-    ( v1 = v2 →
+    ( val_eq v1 v2 →
       envs_entails Δ' (WP fill K #true @ E {{ Φ }})
     ) →
     envs_entails Δ (WP fill K (v1 = v2) @ E {{ Φ }}).
@@ -201,12 +201,25 @@ Section zoo_G.
     iApply ("HΔ'" with "[$Hhdr $Hl $Hmeta]").
   Qed.
 
+  Lemma tac_wp_reveal Δ Δ' K tag vs E Φ :
+    MaybeIntoLaterNEnvs 1 Δ Δ' →
+    ( ∀ bid,
+      envs_entails Δ' (WP fill K (ValBlock (Some bid) tag vs) @ E {{ Φ }})
+    ) →
+    envs_entails Δ (WP fill K (Reveal $ ValBlock None tag vs) @ E {{ Φ }}).
+  Proof.
+    rewrite envs_entails_unseal => HΔ HΔ'.
+    rewrite into_laterN_env_sound -wp_bind -wp_reveal.
+    apply bi.forall_intro => bid.
+    rewrite (HΔ' bid) //.
+  Qed.
+
   Lemma tac_wp_match Δ Δ' id p K l hdr vs x e brs e' E Φ :
     MaybeIntoLaterNEnvs 1 Δ Δ' →
     envs_lookup id Δ' = Some (p, l ↦ₕ hdr)%I →
     envs_entails Δ' (l ↦∗□ vs) →
     length vs = hdr.(header_size) →
-    eval_match (Some l) hdr.(header_tag) vs x e brs = Some e' →
+    eval_match (Some l) None hdr.(header_tag) vs x e brs = Some e' →
     envs_entails Δ' (WP fill K e' @ E {{ Φ }}) →
     envs_entails Δ (WP fill K (Match #l x e brs) @ E {{ Φ }}).
   Proof.
@@ -321,7 +334,7 @@ Section zoo_G.
     ( val_neq v v1 →
       envs_entails Δ' (WP fill K #false @ E {{ Φ }})
     ) →
-    ( v = v1 →
+    ( val_eq v v1 →
       envs_entails Δ' ⌜dq = DfracOwn 1⌝
     ) →
     match
@@ -330,7 +343,7 @@ Section zoo_G.
         Δ''
     with
     | Some Δ''' =>
-        v = v1 →
+        val_eq v v1 →
         envs_entails Δ''' (WP fill K #true @ E {{ Φ }})
     | None =>
         False
@@ -352,7 +365,7 @@ Section zoo_G.
       iDestruct (envs_lookup_sound_2 with "[Hl HΔ'']") as "HΔ'"; [done.. | |].
       { iFrame. destruct p; iSteps. }
       iApply (Hfail with "HΔ'"); first done.
-    - iIntros "!> -> Hl".
+    - iIntros "!> %Heq Hl".
       iDestruct (envs_lookup_sound_2 with "[Hl HΔ'']") as "HΔ'"; [done.. | |].
       { iFrame. destruct p; iSteps. }
       iDestruct (Hsuc1 with "HΔ'") as %->; [done.. |].
@@ -682,6 +695,21 @@ Tactic Notation "wp_ref" ident(l) "as" constr(Hl) :=
   wp_ref l as "_" Hl.
 Tactic Notation "wp_ref" ident(l) :=
   wp_ref l as "?".
+
+Tactic Notation "wp_reveal" simple_intropattern(bid) :=
+  wp_pures;
+  wp_start ltac:(fun e =>
+    first
+    [ reshape_expr e ltac:(fun K e' =>
+        eapply (tac_wp_reveal _ _ K)
+      )
+    | fail 1 "wp_reveal: cannot find 'Reveal' in" e
+    ];
+    [ tc_solve
+    | intros bid;
+      wp_finish
+    ]
+  ).
 
 Tactic Notation "wp_match" open_constr(vs) :=
   wp_pures;
