theories/saturn/mpsc_queue_1.v
@@ -532,12 +532,12 @@ Section mpsc_queue_1_G.
     iDestruct (xchain_model_lookup with "Hhist") as "(Hhist1 & Hnode & Hhist2)"; first done.
     destruct (hist !! S i) as [node' |] eqn:Hlookup'; simpl.
 
-    - wp_cas as _ | [=].
+    - wp_cas as _ | [].
       iDestruct (xchain_model_lookup_2 with "Hhist1 Hnode Hhist2") as "Hhist"; [done | rewrite Hlookup' // |].
       iSplitR "Hnew_back_next Hnew_back_data HΦ". { repeat iExists _. iSteps. }
       iSteps.
 
-    - wp_cas as Hcas | _; first done.
+    - wp_cas as ? | _; first naive_solver.
       iDestruct (xchain_model_lookup_2 with "Hhist1 Hnode []") as "Hhist"; [done | rewrite Hlookup' // | ..].
       { rewrite -(length_lookup_last hist i) // drop_all //. }
       iDestruct (big_sepL2_snoc with "[$Hnodes $Hnew_back_data]") as "Hnodes".
